wip

src/digest.rs
@@ -368,6 +368,12 @@ pub fn shake128<const LEN: usize>(data: &[u8]) -> [u8; LEN] {
 #[cfg_attr(hax, hax_lib_macros::opaque_type)]
 pub struct Shake128State(sha3::incremental::Shake128State);
 
+impl Shake128State {
+    pub fn free(&mut self) {
+        self.0.free()
+    }
+}
+
 pub fn shake128_init() -> Shake128State {
     Shake128State(sha3::incremental::Shake128State::new())
 }
@@ -385,11 +391,6 @@ pub fn shake128_squeeze_nblocks<const OUTPUT_BYTES: usize>(
 ) -> [u8; OUTPUT_BYTES] {
     st.0.squeeze_nblocks()
 }
-
-pub fn shake128_free(mut st: Shake128State) {
-    st.0.free()
-}
-
 /// SHAKE 128 Incremental API (SIMD)
 #[cfg(simd256)]
 #[cfg_attr(hax, hax_lib_macros::opaque_type)]
@@ -414,91 +415,82 @@ pub fn shake128_init_x4() -> Shake128StateX4 {
     ])
 }
 
-#[cfg(simd256)]
-pub fn shake128_free_x4(mut st: Shake128StateX4) {
-    st.0.free()
-}
+// #[cfg(simd256)]
+// pub fn shake128_absorb_nblocks_x4(
+//     st: &mut Shake128StateX4,
+//     data0: &[u8],
+//     data1: &[u8],
+//     data2: &[u8],
+//     data3: &[u8],
+// ) {
+//     st.0.absorb_nblocks(data0, data1, data2, data3);
+// }
 
-#[cfg(not(simd256))]
-pub fn shake128_free_x4(mut st: Shake128StateX4) {
-    st.0[0].free();
-    st.0[1].free();
-    st.0[2].free();
-    st.0[3].free();
-}
+// #[cfg(not(simd256))]
+// pub fn shake128_absorb_nblocks_x4(
+//     st: &mut Shake128StateX4,
+//     data0: &[u8],
+//     data1: &[u8],
+//     data2: &[u8],
+//     data3: &[u8],
+// ) {
+//     st.0[0].absorb_nblocks(data0);
+//     st.0[1].absorb_nblocks(data1);
+//     st.0[2].absorb_nblocks(data2);
+//     st.0[3].absorb_nblocks(data3);
+// }
 
-#[cfg(simd256)]
-pub fn shake128_absorb_nblocks_x4(
-    st: &mut Shake128StateX4,
-    data0: &[u8],
-    data1: &[u8],
-    data2: &[u8],
-    data3: &[u8],
-) {
-    st.0.absorb_nblocks(data0, data1, data2, data3);
-}
+// #[cfg(simd256)]
+// pub fn shake128_absorb_final_x4(
+//     st: &mut Shake128StateX4,
+//     data0: &[u8],
+//     data1: &[u8],
+//     data2: &[u8],
+//     data3: &[u8],
+// ) {
+//     st.0.absorb_final(data0, data1, data2, data3);
+// }
 
-#[cfg(not(simd256))]
-pub fn shake128_absorb_nblocks_x4(
-    st: &mut Shake128StateX4,
-    data0: &[u8],
-    data1: &[u8],
-    data2: &[u8],
-    data3: &[u8],
-) {
-    st.0[0].absorb_nblocks(data0);
-    st.0[1].absorb_nblocks(data1);
-    st.0[2].absorb_nblocks(data2);
-    st.0[3].absorb_nblocks(data3);
-}
+// #[cfg(not(simd256))]
+// pub fn shake128_absorb_final_x4(
+//     st: &mut Shake128StateX4,
+//     data0: &[u8],
+//     data1: &[u8],
+//     data2: &[u8],
+//     data3: &[u8],
+// ) {
+//     st.0[0].absorb_final(data0);
+//     st.0[1].absorb_final(data1);
+//     st.0[2].absorb_final(data2);
+//     st.0[3].absorb_final(data3);
+// }
 
-#[cfg(simd256)]
-pub fn shake128_absorb_final_x4(
-    st: &mut Shake128StateX4,
-    data0: &[u8],
-    data1: &[u8],
-    data2: &[u8],
-    data3: &[u8],
-) {
-    st.0.absorb_final(data0, data1, data2, data3);
-}
+// #[cfg(simd256)]
+// pub fn shake128_squeeze_nblocks_x4<const OUTPUT_BYTES: usize>(
+//     st: &mut Shake128StateX4,
+// ) -> [[u8; OUTPUT_BYTES]; 4] {
+//     st.0.squeeze_nblocks()
+// }
 
-#[cfg(not(simd256))]
-pub fn shake128_absorb_final_x4(
-    st: &mut Shake128StateX4,
-    data0: &[u8],
-    data1: &[u8],
-    data2: &[u8],
-    data3: &[u8],
-) {
-    st.0[0].absorb_final(data0);
-    st.0[1].absorb_final(data1);
-    st.0[2].absorb_final(data2);
-    st.0[3].absorb_final(data3);
-}
-
-#[cfg(simd256)]
-pub fn shake128_squeeze_nblocks_x4<const OUTPUT_BYTES: usize>(
-    st: &mut Shake128StateX4,
-) -> [[u8; OUTPUT_BYTES]; 4] {
-    st.0.squeeze_nblocks()
-}
-
-#[cfg(not(simd256))]
-pub fn shake128_squeeze_nblocks_x4<const OUTPUT_BYTES: usize>(
-    st: &mut Shake128StateX4,
-) -> [[u8; OUTPUT_BYTES]; 4] {
-    let out0: [u8; OUTPUT_BYTES] = st.0[0].squeeze_nblocks();
-    let out1: [u8; OUTPUT_BYTES] = st.0[1].squeeze_nblocks();
-    let out2: [u8; OUTPUT_BYTES] = st.0[2].squeeze_nblocks();
-    let out3: [u8; OUTPUT_BYTES] = st.0[3].squeeze_nblocks();
-    [out0, out1, out2, out3]
-}
+// #[cfg(not(simd256))]
+// pub fn shake128_squeeze_nblocks_x4<const OUTPUT_BYTES: usize>(
+//     st: &mut Shake128StateX4,
+// ) -> [[u8; OUTPUT_BYTES]; 4] {
+//     let out0: [u8; OUTPUT_BYTES] = st.0[0].squeeze_nblocks();
+//     let out1: [u8; OUTPUT_BYTES] = st.0[1].squeeze_nblocks();
+//     let out2: [u8; OUTPUT_BYTES] = st.0[2].squeeze_nblocks();
+//     let out3: [u8; OUTPUT_BYTES] = st.0[3].squeeze_nblocks();
+//     [out0, out1, out2, out3]
+// }
 
 /// SHAKE 128 Incremental API (SIMD)
 #[cfg(simd256)]
 #[cfg_attr(hax, hax_lib_macros::opaque_type)]
 pub struct Shake128StateX2(sha3::incremental_x4::Shake128StateX4);
+
+// #[cfg(not(simd256))]
+// #[cfg_attr(hax, hax_lib_macros::opaque_type)]
+// pub struct Shake128State<const K: usize>([sha3::incremental::Shake128State; K]);
 
 #[cfg(not(simd256))]
 #[cfg_attr(hax, hax_lib_macros::opaque_type)]
@@ -517,58 +509,58 @@ pub fn shake128_init_x2() -> Shake128StateX2 {
     ])
 }
 
-#[cfg(simd256)]
-pub fn shake128_free_x2(mut st: Shake128StateX2) {
-    st.0.free()
-}
+// #[cfg(simd256)]
+// pub fn shake128_free_x2(mut st: Shake128StateX2) {
+//     st.0.free()
+// }
 
-#[cfg(not(simd256))]
-pub fn shake128_free_x2(mut st: Shake128StateX2) {
-    st.0[0].free();
-    st.0[1].free();
-}
+// #[cfg(not(simd256))]
+// pub fn shake128_free_x2(mut st: Shake128StateX2) {
+//     st.0[0].free();
+//     st.0[1].free();
+// }
 
-#[cfg(simd256)]
-pub fn shake128_absorb_nblocks_x2(st: &mut Shake128StateX2, data0: &[u8], data1: &[u8]) {
-    st.0.absorb_nblocks(data0, data1, data0, data1);
-}
+// #[cfg(simd256)]
+// pub fn shake128_absorb_nblocks_x2(st: &mut Shake128StateX2, data0: &[u8], data1: &[u8]) {
+//     st.0.absorb_nblocks(data0, data1, data0, data1);
+// }
 
-#[cfg(not(simd256))]
-pub fn shake128_absorb_nblocks_x2(st: &mut Shake128StateX2, data0: &[u8], data1: &[u8]) {
-    st.0[0].absorb_nblocks(data0);
-    st.0[1].absorb_nblocks(data1);
-}
+// #[cfg(not(simd256))]
+// pub fn shake128_absorb_nblocks_x2(st: &mut Shake128StateX2, data0: &[u8], data1: &[u8]) {
+//     st.0[0].absorb_nblocks(data0);
+//     st.0[1].absorb_nblocks(data1);
+// }
 
-#[cfg(simd256)]
-pub fn shake128_absorb_final_x2(st: &mut Shake128StateX2, data0: &[u8], data1: &[u8]) {
-    st.0.absorb_final(data0, data1, data0, data1);
-}
+// #[cfg(simd256)]
+// pub fn shake128_absorb_final_x2(st: &mut Shake128StateX2, data0: &[u8], data1: &[u8]) {
+//     st.0.absorb_final(data0, data1, data0, data1);
+// }
 
-#[cfg(not(simd256))]
-pub fn shake128_absorb_final_x2(st: &mut Shake128StateX2, data0: &[u8], data1: &[u8]) {
-    st.0[0].absorb_final(data0);
-    st.0[1].absorb_final(data1);
-}
+// #[cfg(not(simd256))]
+// pub fn shake128_absorb_final_x2(st: &mut Shake128StateX2, data0: &[u8], data1: &[u8]) {
+//     st.0[0].absorb_final(data0);
+//     st.0[1].absorb_final(data1);
+// }
 
-#[cfg(simd256)]
-pub fn shake128_squeeze_nblocks_x2<const OUTPUT_BYTES: usize>(
-    st: &mut Shake128StateX2,
-) -> [[u8; OUTPUT_BYTES]; 2] {
-    let mut output = [[0u8; OUTPUT_BYTES]; 2];
-    let tmp = st.0.squeeze_nblocks();
-    output[0] = tmp[0];
-    output[1] = tmp[1];
-    output
-}
+// #[cfg(simd256)]
+// pub fn shake128_squeeze_nblocks_x2<const OUTPUT_BYTES: usize>(
+//     st: &mut Shake128StateX2,
+// ) -> [[u8; OUTPUT_BYTES]; 2] {
+//     let mut output = [[0u8; OUTPUT_BYTES]; 2];
+//     let tmp = st.0.squeeze_nblocks();
+//     output[0] = tmp[0];
+//     output[1] = tmp[1];
+//     output
+// }
 
-#[cfg(not(simd256))]
-pub fn shake128_squeeze_nblocks_x2<const OUTPUT_BYTES: usize>(
-    st: &mut Shake128StateX2,
-) -> [[u8; OUTPUT_BYTES]; 2] {
-    let out0: [u8; OUTPUT_BYTES] = st.0[0].squeeze_nblocks();
-    let out1: [u8; OUTPUT_BYTES] = st.0[1].squeeze_nblocks();
-    [out0, out1]
-}
+// #[cfg(not(simd256))]
+// pub fn shake128_squeeze_nblocks_x2<const OUTPUT_BYTES: usize>(
+//     st: &mut Shake128StateX2,
+// ) -> [[u8; OUTPUT_BYTES]; 2] {
+//     let out0: [u8; OUTPUT_BYTES] = st.0[0].squeeze_nblocks();
+//     let out1: [u8; OUTPUT_BYTES] = st.0[1].squeeze_nblocks();
+//     [out0, out1]
+// }
 
 /// SHAKE 128 Incremental API (SIMD)
 #[cfg(simd256)]
@@ -579,97 +571,97 @@ pub struct Shake128StateX3(sha3::incremental_x4::Shake128StateX4);
 #[cfg_attr(hax, hax_lib_macros::opaque_type)]
 pub struct Shake128StateX3([sha3::incremental::Shake128State; 3]);
 
-#[cfg(simd256)]
-pub fn shake128_init_x3() -> Shake128StateX3 {
-    Shake128StateX3(sha3::incremental_x4::Shake128StateX4::new())
-}
+// #[cfg(simd256)]
+// pub fn shake128_init_x3() -> Shake128StateX3 {
+//     Shake128StateX3(sha3::incremental_x4::Shake128StateX4::new())
+// }
 
-#[cfg(not(simd256))]
-pub fn shake128_init_x3() -> Shake128StateX3 {
-    Shake128StateX3([
-        sha3::incremental::Shake128State::new(),
-        sha3::incremental::Shake128State::new(),
-        sha3::incremental::Shake128State::new(),
-    ])
-}
+// #[cfg(not(simd256))]
+// pub fn shake128_init_x3() -> Shake128StateX3 {
+//     Shake128StateX3([
+//         sha3::incremental::Shake128State::new(),
+//         sha3::incremental::Shake128State::new(),
+//         sha3::incremental::Shake128State::new(),
+//     ])
+// }
 
-#[cfg(simd256)]
-pub fn shake128_free_x3(mut st: Shake128StateX3) {
-    st.0.free()
-}
+// #[cfg(simd256)]
+// pub fn shake128_free_x3(mut st: Shake128StateX3) {
+//     st.0.free()
+// }
 
-#[cfg(not(simd256))]
-pub fn shake128_free_x3(mut st: Shake128StateX3) {
-    st.0[0].free();
-    st.0[1].free();
-    st.0[2].free();
-}
+// #[cfg(not(simd256))]
+// pub fn shake128_free_x3(mut st: Shake128StateX3) {
+//     st.0[0].free();
+//     st.0[1].free();
+//     st.0[2].free();
+// }
 
-#[cfg(simd256)]
-pub fn shake128_absorb_nblocks_x3(
-    st: &mut Shake128StateX3,
-    data0: &[u8],
-    data1: &[u8],
-    data2: &[u8],
-) {
-    st.0.absorb_nblocks(data0, data1, data2, data0);
-}
+// #[cfg(simd256)]
+// pub fn shake128_absorb_nblocks_x3(
+//     st: &mut Shake128StateX3,
+//     data0: &[u8],
+//     data1: &[u8],
+//     data2: &[u8],
+// ) {
+//     st.0.absorb_nblocks(data0, data1, data2, data0);
+// }
 
-#[cfg(not(simd256))]
-pub fn shake128_absorb_nblocks_x3(
-    st: &mut Shake128StateX3,
-    data0: &[u8],
-    data1: &[u8],
-    data2: &[u8],
-) {
-    st.0[0].absorb_nblocks(data0);
-    st.0[1].absorb_nblocks(data1);
-    st.0[2].absorb_nblocks(data2);
-}
+// #[cfg(not(simd256))]
+// pub fn shake128_absorb_nblocks_x3(
+//     st: &mut Shake128StateX3,
+//     data0: &[u8],
+//     data1: &[u8],
+//     data2: &[u8],
+// ) {
+//     st.0[0].absorb_nblocks(data0);
+//     st.0[1].absorb_nblocks(data1);
+//     st.0[2].absorb_nblocks(data2);
+// }
 
-#[cfg(simd256)]
-pub fn shake128_absorb_final_x3(
-    st: &mut Shake128StateX3,
-    data0: &[u8],
-    data1: &[u8],
-    data2: &[u8],
-) {
-    st.0.absorb_final(data0, data1, data2, data0);
-}
+// #[cfg(simd256)]
+// pub fn shake128_absorb_final_x3(
+//     st: &mut Shake128StateX3,
+//     data0: &[u8],
+//     data1: &[u8],
+//     data2: &[u8],
+// ) {
+//     st.0.absorb_final(data0, data1, data2, data0);
+// }
 
-#[cfg(not(simd256))]
-pub fn shake128_absorb_final_x3(
-    st: &mut Shake128StateX3,
-    data0: &[u8],
-    data1: &[u8],
-    data2: &[u8],
-) {
-    st.0[0].absorb_final(data0);
-    st.0[1].absorb_final(data1);
-    st.0[2].absorb_final(data2);
-}
+// #[cfg(not(simd256))]
+// pub fn shake128_absorb_final_x3(
+//     st: &mut Shake128StateX3,
+//     data0: &[u8],
+//     data1: &[u8],
+//     data2: &[u8],
+// ) {
+//     st.0[0].absorb_final(data0);
+//     st.0[1].absorb_final(data1);
+//     st.0[2].absorb_final(data2);
+// }
 
-#[cfg(simd256)]
-pub fn shake128_squeeze_nblocks_x3<const OUTPUT_BYTES: usize>(
-    st: &mut Shake128StateX3,
-) -> [[u8; OUTPUT_BYTES]; 3] {
-    let mut output = [[0u8; OUTPUT_BYTES]; 3];
-    let tmp = st.0.squeeze_nblocks();
-    output[0] = tmp[0];
-    output[1] = tmp[1];
-    output[2] = tmp[2];
-    output
-}
+// #[cfg(simd256)]
+// pub fn shake128_squeeze_nblocks_x3<const OUTPUT_BYTES: usize>(
+//     st: &mut Shake128StateX3,
+// ) -> [[u8; OUTPUT_BYTES]; 3] {
+//     let mut output = [[0u8; OUTPUT_BYTES]; 3];
+//     let tmp = st.0.squeeze_nblocks();
+//     output[0] = tmp[0];
+//     output[1] = tmp[1];
+//     output[2] = tmp[2];
+//     output
+// }
 
-#[cfg(not(simd256))]
-pub fn shake128_squeeze_nblocks_x3<const OUTPUT_BYTES: usize>(
-    st: &mut Shake128StateX3,
-) -> [[u8; OUTPUT_BYTES]; 3] {
-    let out0: [u8; OUTPUT_BYTES] = st.0[0].squeeze_nblocks();
-    let out1: [u8; OUTPUT_BYTES] = st.0[1].squeeze_nblocks();
-    let out2: [u8; OUTPUT_BYTES] = st.0[2].squeeze_nblocks();
-    [out0, out1, out2]
-}
+// #[cfg(not(simd256))]
+// pub fn shake128_squeeze_nblocks_x3<const OUTPUT_BYTES: usize>(
+//     st: &mut Shake128StateX3,
+// ) -> [[u8; OUTPUT_BYTES]; 3] {
+//     let out0: [u8; OUTPUT_BYTES] = st.0[0].squeeze_nblocks();
+//     let out1: [u8; OUTPUT_BYTES] = st.0[1].squeeze_nblocks();
+//     let out2: [u8; OUTPUT_BYTES] = st.0[2].squeeze_nblocks();
+//     [out0, out1, out2]
+// }
 
 /// SHAKE 256
 ///
