src/kem/kyber/hash_functions.rs
@@ -1,6 +1,9 @@
 #![allow(non_snake_case)]
 
-use crate::digest::{self, digest_size, Algorithm};
+use crate::digest::{
+    self, digest_size, shake128_absorb_final, shake128_init, shake128_squeeze_nblocks, Algorithm,
+    Shake128State,
+};
 
 use super::constants::H_DIGEST_SIZE;
 
@@ -16,146 +19,42 @@ pub(crate) fn PRF<const LEN: usize>(input: &[u8]) -> [u8; LEN] {
     digest::shake256::<LEN>(input)
 }
 
-// The following API uses the repeated squeeze API
-// The first version uses Scalar SHAKE 128
-pub(crate) enum XofState {
-    X2(digest::Shake128StateX2),
-    X3(digest::Shake128StateX3),
-    X4(digest::Shake128StateX4),
-}
-
 #[inline(always)]
-pub(crate) fn XOF_absorb<const K: usize>(input: [[u8; 34]; K]) -> XofState {
-    match K as u8 {
-        2 => {
-            let mut state = digest::shake128_init_x2();
-            digest::shake128_absorb_final_x2(&mut state, &input[0], &input[1]);
-            XofState::X2(state)
-        }
-        3 => {
-            let mut state = digest::shake128_init_x3();
-            digest::shake128_absorb_final_x3(&mut state, &input[0], &input[1], &input[2]);
-            XofState::X3(state)
-        }
-        4 => {
-            let mut state = digest::shake128_init_x4();
-            digest::shake128_absorb_final_x4(
-                &mut state, &input[0], &input[1], &input[2], &input[3],
-            );
-            XofState::X4(state)
-        }
-        _ => unreachable!(),
+pub(crate) fn XOF_absorb<const K: usize>(input: [[u8; 34]; K]) -> [Shake128State; K] {
+    let mut state: [Shake128State; K] = core::array::from_fn(|_| shake128_init());
+    // [(); K].map(|_| shake128_init());
+    for i in 0..K {
+        shake128_absorb_final(&mut state[i], &input[i]);
     }
+    state
 }
 
 #[inline(always)]
 pub(crate) fn XOF_squeeze_three_blocks<const K: usize>(
-    xof_state: XofState,
-) -> ([[u8; 168 * 3]; K], XofState) {
+    mut xof_state: [Shake128State; K],
+) -> ([[u8; 168 * 3]; K], [Shake128State; K]) {
     let mut output = [[0; 168 * 3]; K];
-    match K as u8 {
-        2 => {
-            if let XofState::X2(mut st) = xof_state {
-                let tmp = digest::shake128_squeeze_nblocks_x2::<504>(&mut st);
-                output[0] = tmp[0];
-                output[1] = tmp[1];
-                (output, XofState::X2(st))
-            } else {
-                unreachable!()
-            }
-        }
-        3 => {
-            if let XofState::X3(mut st) = xof_state {
-                let tmp = digest::shake128_squeeze_nblocks_x3::<504>(&mut st);
-                output[0] = tmp[0];
-                output[1] = tmp[1];
-                output[2] = tmp[2];
-                (output, XofState::X3(st))
-            } else {
-                unreachable!()
-            }
-        }
-        4 => {
-            if let XofState::X4(mut st) = xof_state {
-                let tmp = digest::shake128_squeeze_nblocks_x4::<504>(&mut st);
-                output[0] = tmp[0];
-                output[1] = tmp[1];
-                output[2] = tmp[2];
-                output[3] = tmp[3];
-                (output, XofState::X4(st))
-            } else {
-                unreachable!()
-            }
-        }
-        _ => unreachable!(),
+    for i in 0..K {
+        output[i] = shake128_squeeze_nblocks(&mut xof_state[i]);
     }
+    (output, xof_state)
 }
 
 #[inline(always)]
-pub(crate) fn XOF_squeeze_block<const K: usize>(xof_state: XofState) -> ([[u8; 168]; K], XofState) {
-    let mut output = [[0; 168]; K];
-    match K as u8 {
-        2 => {
-            if let XofState::X2(mut st) = xof_state {
-                let tmp = digest::shake128_squeeze_nblocks_x2::<168>(&mut st);
-                output[0] = tmp[0];
-                output[1] = tmp[1];
-                (output, XofState::X2(st))
-            } else {
-                unreachable!()
-            }
-        }
-        3 => {
-            if let XofState::X3(mut st) = xof_state {
-                let tmp = digest::shake128_squeeze_nblocks_x3::<168>(&mut st);
-                output[0] = tmp[0];
-                output[1] = tmp[1];
-                output[2] = tmp[2];
-                (output, XofState::X3(st))
-            } else {
-                unreachable!()
-            }
-        }
-        4 => {
-            if let XofState::X4(mut st) = xof_state {
-                let tmp = digest::shake128_squeeze_nblocks_x4::<168>(&mut st);
-                output[0] = tmp[0];
-                output[1] = tmp[1];
-                output[2] = tmp[2];
-                output[3] = tmp[3];
-                (output, XofState::X4(st))
-            } else {
-                unreachable!()
-            }
-        }
-        _ => unreachable!(),
+pub(crate) fn XOF_squeeze_block<const K: usize>(
+    mut xof_state: [Shake128State; K],
+) -> ([[u8; 168]; K], [Shake128State; K]) {
+    let mut output = [[0u8; 168]; K];
+    for i in 0..K {
+        output[i] = shake128_squeeze_nblocks(&mut xof_state[i]);
     }
+
+    (output, xof_state)
 }
 
 #[inline(always)]
-pub(crate) fn XOF_free<const K: usize>(xof_state: XofState) {
-    match K as u8 {
-        2 => {
-            if let XofState::X2(st) = xof_state {
-                digest::shake128_free_x2(st);
-            } else {
-                unreachable!()
-            }
-        }
-        3 => {
-            if let XofState::X3(st) = xof_state {
-                digest::shake128_free_x3(st);
-            } else {
-                unreachable!()
-            }
-        }
-        4 => {
-            if let XofState::X4(st) = xof_state {
-                digest::shake128_free_x4(st);
-            } else {
-                unreachable!()
-            }
-        }
-        _ => unreachable!(),
+pub(crate) fn XOF_free<const K: usize>(mut xof_state: [Shake128State; K]) {
+    for i in 0..K {
+        xof_state[i].free()
     }
 }
