proofs/fstar/extraction/Libcrux.Kem.Kyber.Hash_functions.fst
@@ -10,270 +10,140 @@ let v_H (input: t_Slice u8) = Libcrux.Digest.sha3_256_ input
 let v_PRF (v_LEN: usize) (input: t_Slice u8) = Libcrux.Digest.shake256 v_LEN input
 
 let v_XOF_absorb (v_K: usize) (input: t_Array (t_Array u8 (sz 34)) v_K) =
-  match cast (v_K <: usize) <: u8 with
-  | 2uy ->
-    let state:Libcrux.Digest.t_Shake128StateX2 = Libcrux.Digest.shake128_init_x2 () in
-    let state:Libcrux.Digest.t_Shake128StateX2 =
-      Libcrux.Digest.shake128_absorb_final_x2 state
-        (Rust_primitives.unsize (input.[ sz 0 ] <: t_Array u8 (sz 34)) <: t_Slice u8)
-        (Rust_primitives.unsize (input.[ sz 1 ] <: t_Array u8 (sz 34)) <: t_Slice u8)
-    in
-    XofState_X2 state <: t_XofState
-  | 3uy ->
-    let state:Libcrux.Digest.t_Shake128StateX3 = Libcrux.Digest.shake128_init_x3 () in
-    let state:Libcrux.Digest.t_Shake128StateX3 =
-      Libcrux.Digest.shake128_absorb_final_x3 state
-        (Rust_primitives.unsize (input.[ sz 0 ] <: t_Array u8 (sz 34)) <: t_Slice u8)
-        (Rust_primitives.unsize (input.[ sz 1 ] <: t_Array u8 (sz 34)) <: t_Slice u8)
-        (Rust_primitives.unsize (input.[ sz 2 ] <: t_Array u8 (sz 34)) <: t_Slice u8)
-    in
-    XofState_X3 state <: t_XofState
-  | 4uy ->
-    let state:Libcrux.Digest.t_Shake128StateX4 = Libcrux.Digest.shake128_init_x4 () in
-    let state:Libcrux.Digest.t_Shake128StateX4 =
-      Libcrux.Digest.shake128_absorb_final_x4 state
-        (Rust_primitives.unsize (input.[ sz 0 ] <: t_Array u8 (sz 34)) <: t_Slice u8)
-        (Rust_primitives.unsize (input.[ sz 1 ] <: t_Array u8 (sz 34)) <: t_Slice u8)
-        (Rust_primitives.unsize (input.[ sz 2 ] <: t_Array u8 (sz 34)) <: t_Slice u8)
-        (Rust_primitives.unsize (input.[ sz 3 ] <: t_Array u8 (sz 34)) <: t_Slice u8)
-    in
-    XofState_X4 state <: t_XofState
-  | _ ->
-    Rust_primitives.Hax.never_to_any (Core.Panicking.panic "internal error: entered unreachable code"
-
+  let (state: t_Array Libcrux.Digest.t_Shake128State v_K):t_Array Libcrux.Digest.t_Shake128State v_K
+  =
+    Core.Array.from_fn v_K
+      (fun temp_0_ ->
+          let _:usize = temp_0_ in
+          Libcrux.Digest.shake128_init () <: Libcrux.Digest.t_Shake128State)
+  in
+  let state:t_Array Libcrux.Digest.t_Shake128State v_K =
+    Core.Iter.Traits.Iterator.f_fold (Core.Iter.Traits.Collect.f_into_iter ({
+              Core.Ops.Range.f_start = sz 0;
+              Core.Ops.Range.f_end = v_K
+            }
+            <:
+            Core.Ops.Range.t_Range usize)
         <:
-        Rust_primitives.Hax.t_Never)
+        Core.Ops.Range.t_Range usize)
+      state
+      (fun state i ->
+          let state:t_Array Libcrux.Digest.t_Shake128State v_K = state in
+          let i:usize = i in
+          Rust_primitives.Hax.Monomorphized_update_at.update_at_usize state
+            i
+            (Libcrux.Digest.shake128_absorb_final (state.[ i ] <: Libcrux.Digest.t_Shake128State)
+                (Rust_primitives.unsize (input.[ i ] <: t_Array u8 (sz 34)) <: t_Slice u8)
+              <:
+              Libcrux.Digest.t_Shake128State)
+          <:
+          t_Array Libcrux.Digest.t_Shake128State v_K)
+  in
+  state
 
-let v_XOF_free (v_K: usize) (xof_state: t_XofState) =
-  match cast (v_K <: usize) <: u8 with
-  | 2uy ->
-    (match xof_state with
-      | XofState_X2 st ->
-        let _:Prims.unit = Libcrux.Digest.shake128_free_x2 st in
-        ()
-      | _ ->
-        Rust_primitives.Hax.never_to_any (Core.Panicking.panic "internal error: entered unreachable code"
-
+let v_XOF_free (v_K: usize) (xof_state: t_Array Libcrux.Digest.t_Shake128State v_K) =
+  Core.Iter.Traits.Iterator.f_fold (Core.Iter.Traits.Collect.f_into_iter ({
+            Core.Ops.Range.f_start = sz 0;
+            Core.Ops.Range.f_end = v_K
+          }
+          <:
+          Core.Ops.Range.t_Range usize)
+      <:
+      Core.Ops.Range.t_Range usize)
+    xof_state
+    (fun xof_state i ->
+        let xof_state:t_Array Libcrux.Digest.t_Shake128State v_K = xof_state in
+        let i:usize = i in
+        Rust_primitives.Hax.Monomorphized_update_at.update_at_usize xof_state
+          i
+          (Libcrux.Digest.impl__Shake128State__free (xof_state.[ i ]
+                <:
+                Libcrux.Digest.t_Shake128State)
             <:
-            Rust_primitives.Hax.t_Never))
-  | 3uy ->
-    (match xof_state with
-      | XofState_X3 st ->
-        let _:Prims.unit = Libcrux.Digest.shake128_free_x3 st in
-        ()
-      | _ ->
-        Rust_primitives.Hax.never_to_any (Core.Panicking.panic "internal error: entered unreachable code"
-
-            <:
-            Rust_primitives.Hax.t_Never))
-  | 4uy ->
-    (match xof_state with
-      | XofState_X4 st ->
-        let _:Prims.unit = Libcrux.Digest.shake128_free_x4 st in
-        ()
-      | _ ->
-        Rust_primitives.Hax.never_to_any (Core.Panicking.panic "internal error: entered unreachable code"
-
-            <:
-            Rust_primitives.Hax.t_Never))
-  | _ ->
-    Rust_primitives.Hax.never_to_any (Core.Panicking.panic "internal error: entered unreachable code"
-
+            Libcrux.Digest.t_Shake128State)
         <:
-        Rust_primitives.Hax.t_Never)
+        t_Array Libcrux.Digest.t_Shake128State v_K)
 
-let v_XOF_squeeze_block (v_K: usize) (xof_state: t_XofState) =
+let v_XOF_squeeze_block (v_K: usize) (xof_state: t_Array Libcrux.Digest.t_Shake128State v_K) =
   let output:t_Array (t_Array u8 (sz 168)) v_K =
     Rust_primitives.Hax.repeat (Rust_primitives.Hax.repeat 0uy (sz 168) <: t_Array u8 (sz 168)) v_K
   in
-  match cast (v_K <: usize) <: u8 with
-  | 2uy ->
-    (match xof_state with
-      | XofState_X2 st ->
-        let tmp0, out:(Libcrux.Digest.t_Shake128StateX2 & t_Array (t_Array u8 (sz 168)) (sz 2)) =
-          Libcrux.Digest.shake128_squeeze_nblocks_x2 (sz 168) st
-        in
-        let st:Libcrux.Digest.t_Shake128StateX2 = tmp0 in
-        let tmp:t_Array (t_Array u8 (sz 168)) (sz 2) = out in
-        let output:t_Array (t_Array u8 (sz 168)) v_K =
-          Rust_primitives.Hax.Monomorphized_update_at.update_at_usize output
-            (sz 0)
-            (tmp.[ sz 0 ] <: t_Array u8 (sz 168))
-        in
-        let output:t_Array (t_Array u8 (sz 168)) v_K =
-          Rust_primitives.Hax.Monomorphized_update_at.update_at_usize output
-            (sz 1)
-            (tmp.[ sz 1 ] <: t_Array u8 (sz 168))
-        in
-        output, (XofState_X2 st <: t_XofState) <: (t_Array (t_Array u8 (sz 168)) v_K & t_XofState)
-      | _ ->
-        Rust_primitives.Hax.never_to_any (Core.Panicking.panic "internal error: entered unreachable code"
-
+  let output, xof_state:(t_Array (t_Array u8 (sz 168)) v_K &
+    t_Array Libcrux.Digest.t_Shake128State v_K) =
+    Core.Iter.Traits.Iterator.f_fold (Core.Iter.Traits.Collect.f_into_iter ({
+              Core.Ops.Range.f_start = sz 0;
+              Core.Ops.Range.f_end = v_K
+            }
             <:
-            Rust_primitives.Hax.t_Never))
-  | 3uy ->
-    (match xof_state with
-      | XofState_X3 st ->
-        let tmp0, out:(Libcrux.Digest.t_Shake128StateX3 & t_Array (t_Array u8 (sz 168)) (sz 3)) =
-          Libcrux.Digest.shake128_squeeze_nblocks_x3 (sz 168) st
-        in
-        let st:Libcrux.Digest.t_Shake128StateX3 = tmp0 in
-        let tmp:t_Array (t_Array u8 (sz 168)) (sz 3) = out in
-        let output:t_Array (t_Array u8 (sz 168)) v_K =
-          Rust_primitives.Hax.Monomorphized_update_at.update_at_usize output
-            (sz 0)
-            (tmp.[ sz 0 ] <: t_Array u8 (sz 168))
-        in
-        let output:t_Array (t_Array u8 (sz 168)) v_K =
-          Rust_primitives.Hax.Monomorphized_update_at.update_at_usize output
-            (sz 1)
-            (tmp.[ sz 1 ] <: t_Array u8 (sz 168))
-        in
-        let output:t_Array (t_Array u8 (sz 168)) v_K =
-          Rust_primitives.Hax.Monomorphized_update_at.update_at_usize output
-            (sz 2)
-            (tmp.[ sz 2 ] <: t_Array u8 (sz 168))
-        in
-        output, (XofState_X3 st <: t_XofState) <: (t_Array (t_Array u8 (sz 168)) v_K & t_XofState)
-      | _ ->
-        Rust_primitives.Hax.never_to_any (Core.Panicking.panic "internal error: entered unreachable code"
-
-            <:
-            Rust_primitives.Hax.t_Never))
-  | 4uy ->
-    (match xof_state with
-      | XofState_X4 st ->
-        let tmp0, out:(Libcrux.Digest.t_Shake128StateX4 & t_Array (t_Array u8 (sz 168)) (sz 4)) =
-          Libcrux.Digest.shake128_squeeze_nblocks_x4 (sz 168) st
-        in
-        let st:Libcrux.Digest.t_Shake128StateX4 = tmp0 in
-        let tmp:t_Array (t_Array u8 (sz 168)) (sz 4) = out in
-        let output:t_Array (t_Array u8 (sz 168)) v_K =
-          Rust_primitives.Hax.Monomorphized_update_at.update_at_usize output
-            (sz 0)
-            (tmp.[ sz 0 ] <: t_Array u8 (sz 168))
-        in
-        let output:t_Array (t_Array u8 (sz 168)) v_K =
-          Rust_primitives.Hax.Monomorphized_update_at.update_at_usize output
-            (sz 1)
-            (tmp.[ sz 1 ] <: t_Array u8 (sz 168))
-        in
-        let output:t_Array (t_Array u8 (sz 168)) v_K =
-          Rust_primitives.Hax.Monomorphized_update_at.update_at_usize output
-            (sz 2)
-            (tmp.[ sz 2 ] <: t_Array u8 (sz 168))
-        in
-        let output:t_Array (t_Array u8 (sz 168)) v_K =
-          Rust_primitives.Hax.Monomorphized_update_at.update_at_usize output
-            (sz 3)
-            (tmp.[ sz 3 ] <: t_Array u8 (sz 168))
-        in
-        output, (XofState_X4 st <: t_XofState) <: (t_Array (t_Array u8 (sz 168)) v_K & t_XofState)
-      | _ ->
-        Rust_primitives.Hax.never_to_any (Core.Panicking.panic "internal error: entered unreachable code"
-
-            <:
-            Rust_primitives.Hax.t_Never))
-  | _ ->
-    Rust_primitives.Hax.never_to_any (Core.Panicking.panic "internal error: entered unreachable code"
-
+            Core.Ops.Range.t_Range usize)
         <:
-        Rust_primitives.Hax.t_Never)
+        Core.Ops.Range.t_Range usize)
+      (output, xof_state
+        <:
+        (t_Array (t_Array u8 (sz 168)) v_K & t_Array Libcrux.Digest.t_Shake128State v_K))
+      (fun temp_0_ i ->
+          let output, xof_state:(t_Array (t_Array u8 (sz 168)) v_K &
+            t_Array Libcrux.Digest.t_Shake128State v_K) =
+            temp_0_
+          in
+          let i:usize = i in
+          let tmp0, out:(Libcrux.Digest.t_Shake128State & t_Array u8 (sz 168)) =
+            Libcrux.Digest.shake128_squeeze_nblocks (sz 168)
+              (xof_state.[ i ] <: Libcrux.Digest.t_Shake128State)
+          in
+          let xof_state:t_Array Libcrux.Digest.t_Shake128State v_K =
+            Rust_primitives.Hax.Monomorphized_update_at.update_at_usize xof_state i tmp0
+          in
+          let hoist1:t_Array u8 (sz 168) = out in
+          let hoist2:t_Array (t_Array u8 (sz 168)) v_K =
+            Rust_primitives.Hax.Monomorphized_update_at.update_at_usize output i hoist1
+          in
+          hoist2, xof_state
+          <:
+          (t_Array (t_Array u8 (sz 168)) v_K & t_Array Libcrux.Digest.t_Shake128State v_K))
+  in
+  output, xof_state
+  <:
+  (t_Array (t_Array u8 (sz 168)) v_K & t_Array Libcrux.Digest.t_Shake128State v_K)
 
-let v_XOF_squeeze_three_blocks (v_K: usize) (xof_state: t_XofState) =
+let v_XOF_squeeze_three_blocks (v_K: usize) (xof_state: t_Array Libcrux.Digest.t_Shake128State v_K) =
   let output:t_Array (t_Array u8 (sz 504)) v_K =
     Rust_primitives.Hax.repeat (Rust_primitives.Hax.repeat 0uy (sz 504) <: t_Array u8 (sz 504)) v_K
   in
-  match cast (v_K <: usize) <: u8 with
-  | 2uy ->
-    (match xof_state with
-      | XofState_X2 st ->
-        let tmp0, out:(Libcrux.Digest.t_Shake128StateX2 & t_Array (t_Array u8 (sz 504)) (sz 2)) =
-          Libcrux.Digest.shake128_squeeze_nblocks_x2 (sz 504) st
-        in
-        let st:Libcrux.Digest.t_Shake128StateX2 = tmp0 in
-        let tmp:t_Array (t_Array u8 (sz 504)) (sz 2) = out in
-        let output:t_Array (t_Array u8 (sz 504)) v_K =
-          Rust_primitives.Hax.Monomorphized_update_at.update_at_usize output
-            (sz 0)
-            (tmp.[ sz 0 ] <: t_Array u8 (sz 504))
-        in
-        let output:t_Array (t_Array u8 (sz 504)) v_K =
-          Rust_primitives.Hax.Monomorphized_update_at.update_at_usize output
-            (sz 1)
-            (tmp.[ sz 1 ] <: t_Array u8 (sz 504))
-        in
-        output, (XofState_X2 st <: t_XofState) <: (t_Array (t_Array u8 (sz 504)) v_K & t_XofState)
-      | _ ->
-        Rust_primitives.Hax.never_to_any (Core.Panicking.panic "internal error: entered unreachable code"
-
+  let output, xof_state:(t_Array (t_Array u8 (sz 504)) v_K &
+    t_Array Libcrux.Digest.t_Shake128State v_K) =
+    Core.Iter.Traits.Iterator.f_fold (Core.Iter.Traits.Collect.f_into_iter ({
+              Core.Ops.Range.f_start = sz 0;
+              Core.Ops.Range.f_end = v_K
+            }
             <:
-            Rust_primitives.Hax.t_Never))
-  | 3uy ->
-    (match xof_state with
-      | XofState_X3 st ->
-        let tmp0, out:(Libcrux.Digest.t_Shake128StateX3 & t_Array (t_Array u8 (sz 504)) (sz 3)) =
-          Libcrux.Digest.shake128_squeeze_nblocks_x3 (sz 504) st
-        in
-        let st:Libcrux.Digest.t_Shake128StateX3 = tmp0 in
-        let tmp:t_Array (t_Array u8 (sz 504)) (sz 3) = out in
-        let output:t_Array (t_Array u8 (sz 504)) v_K =
-          Rust_primitives.Hax.Monomorphized_update_at.update_at_usize output
-            (sz 0)
-            (tmp.[ sz 0 ] <: t_Array u8 (sz 504))
-        in
-        let output:t_Array (t_Array u8 (sz 504)) v_K =
-          Rust_primitives.Hax.Monomorphized_update_at.update_at_usize output
-            (sz 1)
-            (tmp.[ sz 1 ] <: t_Array u8 (sz 504))
-        in
-        let output:t_Array (t_Array u8 (sz 504)) v_K =
-          Rust_primitives.Hax.Monomorphized_update_at.update_at_usize output
-            (sz 2)
-            (tmp.[ sz 2 ] <: t_Array u8 (sz 504))
-        in
-        output, (XofState_X3 st <: t_XofState) <: (t_Array (t_Array u8 (sz 504)) v_K & t_XofState)
-      | _ ->
-        Rust_primitives.Hax.never_to_any (Core.Panicking.panic "internal error: entered unreachable code"
-
-            <:
-            Rust_primitives.Hax.t_Never))
-  | 4uy ->
-    (match xof_state with
-      | XofState_X4 st ->
-        let tmp0, out:(Libcrux.Digest.t_Shake128StateX4 & t_Array (t_Array u8 (sz 504)) (sz 4)) =
-          Libcrux.Digest.shake128_squeeze_nblocks_x4 (sz 504) st
-        in
-        let st:Libcrux.Digest.t_Shake128StateX4 = tmp0 in
-        let tmp:t_Array (t_Array u8 (sz 504)) (sz 4) = out in
-        let output:t_Array (t_Array u8 (sz 504)) v_K =
-          Rust_primitives.Hax.Monomorphized_update_at.update_at_usize output
-            (sz 0)
-            (tmp.[ sz 0 ] <: t_Array u8 (sz 504))
-        in
-        let output:t_Array (t_Array u8 (sz 504)) v_K =
-          Rust_primitives.Hax.Monomorphized_update_at.update_at_usize output
-            (sz 1)
-            (tmp.[ sz 1 ] <: t_Array u8 (sz 504))
-        in
-        let output:t_Array (t_Array u8 (sz 504)) v_K =
-          Rust_primitives.Hax.Monomorphized_update_at.update_at_usize output
-            (sz 2)
-            (tmp.[ sz 2 ] <: t_Array u8 (sz 504))
-        in
-        let output:t_Array (t_Array u8 (sz 504)) v_K =
-          Rust_primitives.Hax.Monomorphized_update_at.update_at_usize output
-            (sz 3)
-            (tmp.[ sz 3 ] <: t_Array u8 (sz 504))
-        in
-        output, (XofState_X4 st <: t_XofState) <: (t_Array (t_Array u8 (sz 504)) v_K & t_XofState)
-      | _ ->
-        Rust_primitives.Hax.never_to_any (Core.Panicking.panic "internal error: entered unreachable code"
-
-            <:
-            Rust_primitives.Hax.t_Never))
-  | _ ->
-    Rust_primitives.Hax.never_to_any (Core.Panicking.panic "internal error: entered unreachable code"
-
+            Core.Ops.Range.t_Range usize)
         <:
-        Rust_primitives.Hax.t_Never)
+        Core.Ops.Range.t_Range usize)
+      (output, xof_state
+        <:
+        (t_Array (t_Array u8 (sz 504)) v_K & t_Array Libcrux.Digest.t_Shake128State v_K))
+      (fun temp_0_ i ->
+          let output, xof_state:(t_Array (t_Array u8 (sz 504)) v_K &
+            t_Array Libcrux.Digest.t_Shake128State v_K) =
+            temp_0_
+          in
+          let i:usize = i in
+          let tmp0, out:(Libcrux.Digest.t_Shake128State & t_Array u8 (sz 504)) =
+            Libcrux.Digest.shake128_squeeze_nblocks (sz 504)
+              (xof_state.[ i ] <: Libcrux.Digest.t_Shake128State)
+          in
+          let xof_state:t_Array Libcrux.Digest.t_Shake128State v_K =
+            Rust_primitives.Hax.Monomorphized_update_at.update_at_usize xof_state i tmp0
+          in
+          let hoist3:t_Array u8 (sz 504) = out in
+          let hoist4:t_Array (t_Array u8 (sz 504)) v_K =
+            Rust_primitives.Hax.Monomorphized_update_at.update_at_usize output i hoist3
+          in
+          hoist4, xof_state
+          <:
+          (t_Array (t_Array u8 (sz 504)) v_K & t_Array Libcrux.Digest.t_Shake128State v_K))
+  in
+  output, xof_state
+  <:
+  (t_Array (t_Array u8 (sz 504)) v_K & t_Array Libcrux.Digest.t_Shake128State v_K)
