proofs/fstar/extraction/Libcrux.Kem.Kyber.Hash_functions.fsti
@@ -10,23 +10,18 @@ val v_H (input: t_Slice u8) : Prims.Pure (t_Array u8 (sz 32)) Prims.l_True (fun 
 val v_PRF (v_LEN: usize) (input: t_Slice u8)
     : Prims.Pure (t_Array u8 v_LEN) Prims.l_True (fun _ -> Prims.l_True)
 
-type t_XofState =
-  | XofState_X2 : Libcrux.Digest.t_Shake128StateX2 -> t_XofState
-  | XofState_X3 : Libcrux.Digest.t_Shake128StateX3 -> t_XofState
-  | XofState_X4 : Libcrux.Digest.t_Shake128StateX4 -> t_XofState
-
 val v_XOF_absorb (v_K: usize) (input: t_Array (t_Array u8 (sz 34)) v_K)
-    : Prims.Pure t_XofState Prims.l_True (fun _ -> Prims.l_True)
+    : Prims.Pure (t_Array Libcrux.Digest.t_Shake128State v_K) Prims.l_True (fun _ -> Prims.l_True)
 
-val v_XOF_free (v_K: usize) (xof_state: t_XofState)
-    : Prims.Pure Prims.unit Prims.l_True (fun _ -> Prims.l_True)
+val v_XOF_free (v_K: usize) (xof_state: t_Array Libcrux.Digest.t_Shake128State v_K)
+    : Prims.Pure (t_Array Libcrux.Digest.t_Shake128State v_K) Prims.l_True (fun _ -> Prims.l_True)
 
-val v_XOF_squeeze_block (v_K: usize) (xof_state: t_XofState)
-    : Prims.Pure (t_Array (t_Array u8 (sz 168)) v_K & t_XofState)
+val v_XOF_squeeze_block (v_K: usize) (xof_state: t_Array Libcrux.Digest.t_Shake128State v_K)
+    : Prims.Pure (t_Array (t_Array u8 (sz 168)) v_K & t_Array Libcrux.Digest.t_Shake128State v_K)
       Prims.l_True
       (fun _ -> Prims.l_True)
 
-val v_XOF_squeeze_three_blocks (v_K: usize) (xof_state: t_XofState)
-    : Prims.Pure (t_Array (t_Array u8 (sz 504)) v_K & t_XofState)
+val v_XOF_squeeze_three_blocks (v_K: usize) (xof_state: t_Array Libcrux.Digest.t_Shake128State v_K)
+    : Prims.Pure (t_Array (t_Array u8 (sz 504)) v_K & t_Array Libcrux.Digest.t_Shake128State v_K)
       Prims.l_True
       (fun _ -> Prims.l_True)
